driver/PolOpt.v
@@ -21,6 +21,8 @@ Require Import SelectionSort.
 
 Require Import Extractor.
 Require Import CodeGen. 
+Require Import PrepareCodegen.
+Require Import StrengthenDomain.
 
 Require Import Validator.
 Require Import LibTactics.
@@ -94,6 +96,8 @@ Definition ident := Instr.ident.
 
 Module Extractor := Extractor PolIRs.
 Module CodeGen := CodeGen PolIRs.
+Module Prepare := PrepareCodegen PolIRs.
+Module Strengthen := StrengthenDomain PolIRs.
 Module Validator := Validator PolIRs.
 (* Definition codegen (pol: Pol.t): result Loop.t := 
    Okk Loop.dummy. *)
@@ -113,7 +117,7 @@ Definition scheduler' (pol: PolIRs.PolyLang.t): imp PolIRs.PolyLang.t :=
    end.
 
 
-Definition Opt (loop: PolIRs.Loop.t): imp PolIRs.Loop.t := 
+Definition Opt_raw (loop: PolIRs.Loop.t): imp PolIRs.Loop.t := 
    pure loop
    @@@[PolIRs.PolyLang.dummy] time "PolOpt.Extractor" Extractor.extractor
    (* @@ print (print_CPol) *)
@@ -172,6 +176,116 @@ Proof.
    split; eauto.
    eapply State.eq_trans; eauto.
 Qed.   
+
+Definition Opt_prepared (loop: Loop.t): imp Loop.t :=
+  BIND pol0 <- res_to_alarm PolyLang.dummy (Extractor.extractor loop) -;
+  BIND pol' <- scheduler' (Strengthen.strengthen_pprog pol0) -;
+  Prepare.prepared_codegen pol'.
+
+Definition Opt : Loop.t -> imp Loop.t := Opt_prepared.
+
+Lemma extractor_success_wf_pprog:
+  forall loop pol,
+    Extractor.extractor loop = Okk pol ->
+    PolyLang.wf_pprog pol.
+Proof.
+  intros loop [[pis varctxt] vars] Hext.
+  split.
+  - eapply Extractor.extractor_success_implies_varctxt_le_vars; eauto.
+  - intros pi Hin.
+    pose proof (Extractor.extractor_success_implies_wf_pinstrs loop pis varctxt vars Hext) as Hall.
+    eapply Forall_forall in Hall; eauto.
+Qed.
+
+Lemma scheduler'_preserve_wf:
+  forall pol pol',
+    PolyLang.wf_pprog pol ->
+    WHEN pol'' <- scheduler' pol THEN
+    pol'' = pol' ->
+    PolyLang.wf_pprog pol'.
+Proof.
+  intros pol pol' Hwf pol'' Hsched Heq.
+  subst pol''.
+  unfold scheduler' in Hsched.
+  destruct scheduler eqn:Hschedsrc.
+  2: {
+    exfalso.
+    eapply mayReturn_alarm in Hsched.
+    exact Hsched.
+  }
+  bind_imp_destruct Hsched res Hval.
+  destruct res.
+  2: {
+    exfalso.
+    eapply mayReturn_alarm in Hsched.
+    exact Hsched.
+  }
+  eapply mayReturn_pure in Hsched. subst.
+  pose proof (Validator.validate_preserve_wf_pprog pol pol' _ Hval eq_refl) as [_ Hwf'].
+  exact Hwf'.
+Qed.
+
+Theorem Extract_Schedule_Prepared_correct:
+  forall loop pol st1 st2,
+    Extractor.extractor loop = Okk pol ->
+    WHEN pol' <- scheduler' (Strengthen.strengthen_pprog pol) THEN
+    PolyLang.wf_pprog pol' ->
+    PolyLang.semantics (Prepare.prepare_codegen pol') st1 st2 ->
+    exists st2',
+      Loop.semantics loop st1 st2' /\ State.eq st2 st2'.
+Proof.
+  intros loop pol st1 st2 Hext pol' Hsched Hwf Hsem.
+  eapply Prepare.prepare_codegen_semantics_correct in Hsem; eauto.
+  pose proof (scheduler'_correct (Strengthen.strengthen_pprog pol) st1 st2 pol' Hsched Hsem)
+    as Hsched_corr.
+  destruct Hsched_corr as [st_mid [Hips Heq]].
+  eapply Strengthen.instance_list_semantics_unstrengthen in Hips.
+  pose proof (Extractor.extractor_correct loop pol st1 st_mid Hext Hips) as Hext_corr.
+  destruct Hext_corr as [st_src [Hloop Heq_src]].
+  exists st_src. split; auto.
+  eapply State.eq_trans; eauto.
+Qed.
+
+Theorem Opt_prepared_correct:
+  forall loop st st',
+    WHEN loop' <- Opt_prepared loop THEN
+    Loop.semantics loop' st st' ->
+    exists st'',
+      Loop.semantics loop st st'' /\ State.eq st' st''.
+Proof.
+  intros loop st st' loop' Hopt Hloop.
+  unfold Opt_prepared in Hopt.
+  bind_imp_destruct Hopt pol0 Hextimp.
+  bind_imp_destruct Hopt pol' Hsched.
+  apply res_to_alarm_correct in Hextimp.
+  assert (Hwfpol' : PolyLang.wf_pprog pol').
+  {
+    eapply scheduler'_preserve_wf.
+    - eapply Strengthen.strengthen_pprog_wf.
+      eapply extractor_success_wf_pprog; eauto.
+    - exact Hsched.
+    - reflexivity.
+  }
+  pose proof (Prepare.prepared_codegen_correct pol' st st' loop' Hopt Hwfpol' Hloop) as Hips.
+  pose proof (scheduler'_correct (Strengthen.strengthen_pprog pol0) st st' pol' Hsched Hips)
+    as Hsched_corr.
+  destruct Hsched_corr as [st_mid [Hips' Heq]].
+  eapply Strengthen.instance_list_semantics_unstrengthen in Hips'.
+  pose proof (Extractor.extractor_correct loop pol0 st st_mid Hextimp Hips') as Hext_corr.
+  destruct Hext_corr as [st_src [Hloop_src Heq_src]].
+  exists st_src. split; auto.
+  eapply State.eq_trans; eauto.
+Qed.
+
+Theorem Opt_correct:
+  forall loop st st',
+    WHEN loop' <- Opt loop THEN
+    Loop.semantics loop' st st' ->
+    exists st'',
+      Loop.semantics loop st st'' /\ State.eq st' st''.
+Proof.
+  exact Opt_prepared_correct.
+Qed.
 
 Close Scope impure_scope.
 Close Scope opt_scop.
